proofs/itrees/it_sems_mden1.v
@@ -1,0 +1,986 @@
+
+From ITree Require Import
+     Basics
+     ITree
+     ITreeFacts
+     Events.Exception
+     Interp.Recursion
+     MonadState
+     State
+     StateFacts.
+Import Basics.Monads.
+
+From mathcomp Require Import ssreflect ssrfun ssrbool eqtype.
+
+Require Import expr psem_defs psem_core it_exec it_sems_exec tfam_iso1.
+
+Import MonadNotation.
+Local Open Scope monad_scope.
+
+Section Asm1.  
+Context
+  {asm_op: Type} {asmop: asmOp asm_op}.
+(*
+Context
+  {asm_op: Type}
+  {syscall_state : Type}
+  {sip : SemInstrParams asm_op syscall_state}.  
+  {wsw: WithSubWord} 
+  {dc: DirectCall} 
+  {ep : EstateParams syscall_state} 
+  {spp : SemPexprParams} 
+  {pT : progT}
+  {scP : semCallParams}. *)
+
+Section Sem1.
+Context (FState : Type) {State: Type} {FunDef: Type}.
+Context {err: error_data}.
+
+Local Notation continue_loop := (ret (inl tt)).
+Local Notation exit_loop := (ret (inr tt)).
+Local Notation rec_call := (trigger_inl1). 
+
+(* mutual recursion events (corresponding to call states) *)
+Variant MREvent : Type -> Type :=
+  | LCode (c: cmd) : MREvent unit
+  | FCall (fn: funname) (fs: FState) : MREvent FState.
+
+(* state events (similar to those provided by the library, 
+   could be specialized to estate) *)
+Variant StE : Type -> Type :=
+  | GetSE : StE State
+  | PutSE : State -> StE unit.                      
+
+(* instruction events *)
+Variant InstrE : Type -> Type :=
+  | AssgnE : lval -> assgn_tag -> stype -> pexpr -> InstrE unit
+  | OpnE : lvals -> assgn_tag -> sopn -> pexprs -> InstrE unit
+  | SyscallE : lvals -> syscall_t -> pexprs -> InstrE unit
+  | EvalCond (e: pexpr) : InstrE bool
+  | EvalBound (e: pexpr) : InstrE Z
+  | WriteIndex (x: var_i) (z: Z) : InstrE unit
+  | EvalArgs (args: pexprs) : InstrE pexprs                
+  | InitFState (args: pexprs) : InstrE FState
+  | RetVal (xs: lvals) (fs: FState) (s: State) : InstrE unit.
+
+(* function call events *)
+Variant FunE : Type -> Type :=
+  | GetFunDef (fn: funname) (fs: FState) : FunE FunDef
+  | GetFunCode (fd: FunDef) : FunE cmd          
+  | InitFunCall (fd: FunDef) (fs: FState) : FunE FState                     
+  | FinalizeFunCall (fd: FunDef) : FunE FState.
+
+(* folding instruction semantics on commands 
+   (without state, it could be simply map) *)
+Definition isem_foldr {E} (sem_i: instr -> itree E unit) (c: cmd) :
+    itree E unit :=
+  foldr (fun i k => sem_i i ;; k) (Ret tt) c.
+
+Definition isem_for_round {E} (sem_i: instr -> itree E unit)
+  (wrt: Z -> itree E unit)                        
+  (i : var_i) (c : cmd) (w: Z) (k: itree E unit) : itree E unit :=
+  wrt w ;; isem_foldr sem_i c ;; k.
+
+Definition isem_for_loop  {E} (sem_i: instr -> itree E unit)
+  (wrt: Z -> itree E unit) 
+  (i : var_i) (c : cmd) (ls : list Z)
+  : itree E unit :=
+  foldr (isem_for_round sem_i wrt i c) (Ret tt) ls.
+
+Definition isem_while_round {E} (sem_i: instr -> itree E unit)
+  (cnd: pexpr -> itree E bool) 
+  (c1 : cmd) (e : pexpr) (c2 : cmd) :
+    itree E (unit + unit) :=
+  isem_foldr sem_i c1 ;;
+  b <- cnd e ;;
+  if b then isem_foldr sem_i c2 ;; continue_loop 
+  else exit_loop.
+
+Definition isem_while_loop {E} (sem_i: instr -> itree E unit)
+  (cnd: pexpr -> itree E bool)
+  (c1 : cmd) (e: pexpr) (c2: cmd) :
+    itree E unit :=
+  ITree.iter (fun _ => isem_while_round sem_i cnd c1 e c2) tt.
+
+
+Section Sem2.
+
+Context {E}
+  {XE : ErrEvent -< E} {XI : InstrE -< E} {XS: StE -< E} {XF: FunE -< E}.
+  
+(* semantics of instructions *)
+Fixpoint esem_instr  
+  (i : instr) : itree (MREvent +' E) unit :=  
+  let R := isem_foldr esem_instr in
+  let: (MkI ii ir) := i in 
+  match ir with
+
+  | Cassgn x tg ty e => trigger (AssgnE x tg ty e)
+                                
+  | Copn xs tg o es => trigger (OpnE xs tg o es)
+                               
+  | Csyscall xs o es => trigger (SyscallE xs o es)
+        
+  | Cif e c1 c2 =>
+    b <- trigger (EvalCond e) ;; 
+    R (if b then c1 else c2)
+
+  | Cwhile a c1 e i c2 =>
+      isem_while_loop esem_instr (fun e => trigger (EvalCond e))
+        c1 e c2 
+        
+  | Cfor i (d, lo, hi) c =>
+    lo_b <- trigger (EvalBound lo) ;;
+    hi_b <- trigger (EvalBound hi) ;;   
+    isem_for_loop esem_instr (fun w => trigger (WriteIndex i (Vint w)))
+      i c (wrange d lo_b hi_b) 
+
+  | Ccall xs fn args =>
+    s0 <- trigger GetSE ;;  
+    vargs <- trigger (EvalArgs args) ;;
+    fs0 <- trigger (InitFState vargs) ;;
+    fs1 <- rec_call (FCall fn fs0) ;; 
+    (* discard current state, use s0 instead *)
+    trigger (RetVal xs fs1 s0)
+(* | _ => throw err end. *)
+  end.
+
+(* semantics of commands *)
+Definition esem_cmd c := isem_foldr esem_instr c.
+
+(* semantics of function calls *)
+Definition esem_fcall (fn : funname) (fs : FState) :
+  itree (MREvent +' E) FState :=
+  fd <- trigger (GetFunDef fn fs) ;;  
+  c <- trigger (GetFunCode fd) ;;
+  trigger (InitFunCall fd fs) ;;
+  rec_call (LCode c) ;;
+  trigger (FinalizeFunCall fd).
+
+(* call state handler *)
+Definition esem_cstate : MREvent ~> itree (MREvent +' E) :=           
+  fun _ fs => match fs with
+              | LCode c => esem_cmd c 
+              | FCall fn fs => esem_fcall fn fs     
+              end.      
+
+(* actual recursive semantics *)
+Definition mrec_cmd (c: cmd) : itree E unit :=
+  mrec esem_cstate (LCode c).
+
+(**********************************************************************)
+
+Definition esem_cstate_blank : MREvent ~> itree (MREvent +' E) :=           
+  fun _ fs => match fs with
+              | LCode c => esem_cmd c 
+              | FCall fn fs => rec_call (FCall fn fs)     
+              end.      
+
+(* blank recursive semantics: does not interpret recursive calls *)
+Definition mrec_cmd_blank (c: cmd) : itree E unit :=
+  mrec esem_cstate_blank (LCode c).
+
+End Sem2.
+
+End Sem1.
+
+End Asm1.
+
+(********************* garbage **********)
+
+From Jasmin Require Import oseq.
+(* problematic *)
+From Jasmin Require Import expr.
+(* From Jasmin Require Import it_jasmin_lib. *)
+
+From Coq Require Import
+     Arith.PeanoNat
+     Lists.List
+     Strings.String
+     Morphisms
+     Setoid
+     RelationClasses
+     EquivDec
+     Equality
+     Program.Tactics.
+
+From ExtLib Require Import
+     Data.String
+     Structures.Monad
+     Structures.Traversable
+     Data.List
+     Core.RelDec
+     Structures.Maps
+     Data.Map.FMapAList.
+
+From ITree Require Import
+     ITree
+     ITreeFacts
+     Monad
+     Basics.HeterogeneousRelations     
+     Events.Map
+     Events.State
+     Events.StateFacts
+     Events.Reader
+     Events.Exception
+     Events.FailFacts.
+
+Require Import Paco.paco.
+Require Import Psatz.
+Require Import ProofIrrelevance.
+Require Import FunctionalExtensionality.
+
+From mathcomp Require Import ssreflect ssrfun ssrbool ssrnat seq eqtype fintype.
+
+From ITree Require Import
+(*     Basics.Tacs *)
+     Basics.Category
+     Basics.Basics
+     Basics.Function
+     Core.ITreeDefinition
+     Core.KTree
+     Eq.Eqit
+     Eq.UpToTaus
+     Eq.Paco2
+     Indexed.Sum
+     Indexed.Function
+     Indexed.Relation
+     Interp.Handler
+     Interp.Interp
+     Interp.InterpFacts
+     Interp.Recursion.
+
+From Jasmin Require Import expr psem_defs psem oseq.
+(* From Jasmin Require Import it_gen_lib it_jasmin_lib. *)
+From Jasmin Require Import compiler_util.
+(* problematic *)
+From Jasmin Require Import it_exec2.
+
+(********************************************************)
+(* TODO: clean up imports above this line *)
+
+From mathcomp Require Import ssreflect ssrfun ssrbool.
+
+Require Import xrutt xrutt_facts. 
+
+Import ITreeNotations.
+Local Open Scope itree_scope.
+
+Import Monads.
+Import MonadNotation.
+Local Open Scope monad_scope.
+Local Open Scope option_scope.
+
+Set Implicit Arguments.
+Unset Strict Implicit.
+Unset Printing Implicit Defensive.
+
+Obligation Tactic := done || idtac.
+
+(*** SEMANTICS + ARRAY INIT *)
+
+(************************************************************************)
+(** from JLang7.v *)
+
+Definition opt_fmap {A B} (f: A -> B) : option A -> option B :=
+  fun m => match m with
+           | Some x => Some (f x) | _ => None end.  
+
+(*
+Definition opt_map {A B} (f: A -> B) : option (list A) -> option (list B) :=
+  opt_fmap (List.map f).
+
+Definition opt_write {S} {V} (ms: option S) (v: V) :
+  option (S * V) :=
+  match ms with  
+  | Some st' => Some (st', v)
+  | _ => None end.    
+
+Definition lift_rel {T} (R: T -> T -> Prop) : option T -> option T -> Prop :=
+  fun x y => match (x, y) with
+             | (Some x', Some y') => R x' y'
+             | (None, None) => True
+             | _ => False end.  
+*)
+
+(**** ERROR SEMANTICS *******************************************)
+Section Errors.
+
+Definition ErrEvent : Type -> Type := exceptE error_data.
+
+(* failT (itree E) R = itree E (option R) *)
+Definition handle_Err {E} : ErrEvent ~> failT (itree E) :=
+  fun _ _ => Ret (None).
+
+(* Err handler *)
+Definition ext_handle_Err {E: Type -> Type} :
+  ErrEvent +' E ~> failT (itree E) :=
+  fun _ e =>
+  match e with
+  | inl1 e' => handle_Err e'
+  | inr1 e' => Vis e' (pure (fun x => Some x)) end.                        
+
+(* ErrEvent interpreter *)
+Definition interp_Err {E: Type -> Type} {A}  
+  (t: itree (ErrEvent +' E) A) : failT (itree E) A :=
+  interp_fail ext_handle_Err t.
+
+(*** auxiliary error functions *)
+
+Definition err_f_get {E: Type -> Type} `{ErrEvent -< E} {S} {V}
+  (err: error_data) (f: S -> option V) : stateT S (itree E) V :=
+  fun st => match (f st) with
+            | Some v => Ret (st, v)
+            | None => throw err end.                
+
+Definition err_f_put {E: Type -> Type} `{ErrEvent -< E} {S}
+  (err : error_data) (f: S -> option S) : stateT S (itree E) unit :=
+  fun st => match (f st) with
+            | Some st' => Ret (st', tt)
+            | None => throw err end.                
+
+Definition err_opt {E: Type -> Type} `{ErrEvent -< E} (err : error_data) :
+  option ~> itree E :=
+  fun _ t => match t with
+             | Some v => Ret v
+             | None => throw err end.                
+
+Definition err_result {E: Type -> Type} `{ErrEvent -< E} T (err : error_data) :
+  result T ~> itree E :=
+  fun _ t => match t with
+             | Ok v => Ret v
+             | Error _ => throw err end.                
+
+End Errors.
+
+
+(*********************************************************************)
+(*** LANGUAGE DEFINITION *********************************************)
+
+Section WSW.
+Context (asm_op: Type) (asmop: asmOp asm_op).
+Context {wsw: WithSubWord}.   
+Context
+  (dc: DirectCall)
+  (syscall_state : Type)
+  (ep : EstateParams syscall_state)
+  (spp : SemPexprParams)
+  (sip : SemInstrParams asm_op syscall_state)
+  (pT : progT)
+  (scP : semCallParams)
+  (ev : extra_val_t).
+  
+Context (pr : prog).
+
+(* default error *)  
+Context (err: error_data).
+
+
+(***** FUN-READER SEMANTICS ******************************************)
+Section ModularSem.
+
+(* Analysis info *)  
+Context (AInfo: Type).
+Context (empty_ainfo : AInfo).
+Context (ainfo_updt : instr_info -> AInfo -> AInfo).
+
+Notation ainfo_estate := (AInfo * estate)%type.
+Notation ainfo_bool := (AInfo * bool)%type.
+Notation ainfo_Z := (AInfo * Z)%type.
+Notation ainfo_values := (AInfo * values)%type.
+
+Definition FunDef : Type := _fundef extra_fun_t.
+
+Definition get_FunDef (fn: funname) : option FunDef :=
+  get_fundef (p_funcs pr) fn.
+
+Definition funCode (f: FunDef) : cmd := 
+  @f_body asm_op asmop extra_fun_t f.
+
+Definition get_FunCode (fn: funname) : option cmd := 
+  opt_fmap (@f_body asm_op asmop extra_fun_t) (get_FunDef fn).
+
+Definition get_FunDests (fn: funname) : option lvals :=
+  get_FunDef fn >>= fun f => Some (map Lvar (f.(f_res))). 
+
+
+(***** INSTR AUX FUNCTIONS *******************************************)
+
+(* option to execS *)
+Definition o2xs {aT : Type} (o: option aT) : execS aT :=
+match o with
+| Some x => ESok x
+| None => ESerror _ err
+end.
+
+(* result to execS *)
+Definition r2xs {eT aT : Type} (o: result eT aT) : execS aT :=
+match o with
+| Ok x => ESok x
+| Error _ => ESerror _ err
+end.
+
+(* option to execS with ainfo *)
+Definition o2aixs {aT : Type} (ai: AInfo) (o: option aT) :
+  execS (AInfo * aT) :=
+match o with
+| Some x => ESok (ai, x)
+| None => ESerror _ err
+end.
+Definition o2axs {aT : Type} (o: option aT) := o2aixs empty_ainfo o.
+
+(* result to execS with ainfo *) 
+Definition r2aixs {eT aT : Type} (ai: AInfo) (o: result eT aT) :
+  execS (AInfo * aT) :=
+match o with
+| Ok x => ESok (ai, x)
+| Error _ => ESerror _ err
+end.
+Definition r2axs {eT aT : Type} (o: result eT aT) := r2aixs empty_ainfo o.
+
+Definition o2aio {T} : AInfo -> option T -> option (AInfo * T) :=
+  fun ai o => match o with
+           | Some y => Some (ai, y)
+           | None => None end.                 
+Definition o_add_info {T} (o: option T) := o2aio empty_ainfo o.       
+
+Definition r2air {eT aT} :
+  AInfo -> result eT aT -> result eT (AInfo * aT) :=
+  fun ai x => match x with
+           | Ok y => ok (ai, y)
+           | Error e => Error e end.                 
+Definition r_add_info T (x: exec T) : exec (AInfo * T) :=
+  r2air empty_ainfo x.
+
+
+(******************************************************)
+
+Definition ret_get_FunDef {E: Type -> Type} 
+  (fn: funname) : execT (itree E) FunDef :=
+  Ret (o2xs (get_FunDef fn)).           
+
+Definition ret_get_FunDef' {E: Type -> Type} 
+  (fn: funname) : execT (itree E) (AInfo * FunDef) :=
+  Ret (o2axs (get_FunDef fn)).           
+
+Definition err_get_FunDef {E} `{ErrEvent -< E}
+  (fn: funname) : itree E FunDef :=
+  err_opt err (get_FunDef fn).           
+
+Definition err_get_FunDef' {E} `{ErrEvent -< E}
+  (fn: funname) : itree E (AInfo * FunDef) :=
+  err_opt err (o_add_info (get_FunDef fn)).           
+
+Definition ret_get_FunCode {E: Type -> Type}
+  (fn: funname) : execT (itree E) cmd :=
+  f <- ret_get_FunDef fn ;;
+  Ret (ESok (funCode f)).
+
+Definition ret_get_FunCode' {E: Type -> Type}
+  (fn: funname) : execT (itree E) (AInfo * cmd) :=
+  f <- ret_get_FunDef fn ;;
+  Ret (ESok (empty_ainfo, funCode f)).
+
+Definition err_get_FunCode {E} `{ErrEvent -< E}
+  (fn: funname) : itree E cmd :=
+  f <- err_get_FunDef fn ;;
+  Ret (funCode f).
+
+Definition err_get_FunCode' {E} `{ErrEvent -< E}
+  (fn: funname) : itree E (AInfo * cmd) :=
+  f <- err_get_FunDef fn ;;
+  Ret (empty_ainfo, funCode f).
+
+(******************)
+
+Definition pure_eval_Args (args: pexprs) (st: estate) :
+  exec (seq value) := 
+  sem_pexprs (~~direct_call) (p_globs pr) st args.
+
+Definition truncate_Args (f: FunDef) (vargs: seq value) :
+  exec (seq value) :=
+  mapM2 ErrType dc_truncate_val f.(f_tyin) vargs.
+
+Definition err_eval_Args {E} `{ErrEvent -< E}
+  (fn: funname) (args: pexprs) (st0: estate) : itree E values :=
+  f <- err_get_FunDef fn ;;
+  vargs' <- err_result err (pure_eval_Args args st0) ;;
+  err_result err (truncate_Args f vargs').
+
+Definition err_eval_Args' {E} `{ErrEvent -< E}
+  (fn: funname) (args: pexprs) (st0: ainfo_estate) : itree E ainfo_values :=
+  f <- err_get_FunDef fn ;;
+  vargs' <- err_result err (pure_eval_Args args (snd st0)) ;;
+  err_result err (r_add_info (truncate_Args f vargs')).
+ 
+Definition err_init_state {E} `{ErrEvent -< E}
+   (fn: funname) (vargs: seq value) (st0: estate) : itree E estate :=   
+  let scs1 := st0.(escs) in
+  let m1 := st0.(emem) in
+  f <- err_get_FunDef fn ;;
+  st1 <- err_result err 
+       (init_state f.(f_extra) (p_extra pr) ev (Estate scs1 m1 Vm.init)) ;;
+  err_result err
+      (write_vars (~~direct_call) (f_params f) vargs st1).
+
+Definition err_init_state' {E} `{ErrEvent -< E}
+   (fn: funname) (vargs: seq value) (st0: estate) : itree E ainfo_estate :=   
+  let scs1 := st0.(escs) in
+  let m1 := st0.(emem) in
+  f <- err_get_FunDef fn ;;
+  st1 <- err_result err 
+       (init_state f.(f_extra) (p_extra pr) ev (Estate scs1 m1 Vm.init)) ;;
+  err_result err
+      (r_add_info (write_vars (~~direct_call) (f_params f) vargs st1)).
+
+Definition err_return_val {E} `{ErrEvent -< E}
+  (fn: funname) (st0: estate) : itree E values :=
+  f <- err_get_FunDef fn ;;
+  vres <- err_result err 
+      (get_var_is (~~ direct_call) st0.(evm) f.(f_res)) ;;
+  err_result err
+      (mapM2 ErrType dc_truncate_val f.(f_tyout) vres).
+
+Definition err_return_val' {E} `{ErrEvent -< E}
+  (fn: funname) (st0: estate) : itree E ainfo_values :=
+  f <- err_get_FunDef fn ;;
+  vres <- err_result err 
+      (get_var_is (~~ direct_call) st0.(evm) f.(f_res)) ;;
+  err_result err
+     (r_add_info (mapM2 ErrType dc_truncate_val f.(f_tyout) vres)).
+
+
+Definition err_reinstate_caller {E} `{ErrEvent -< E}
+  (fn: funname) (xs: lvals) (vres: values)
+  (st_ee st_er: estate) : itree E estate :=
+  f <- err_get_FunDef fn ;;
+  let scs2 := st_ee.(escs) in
+  let m2 := finalize f.(f_extra) st_ee.(emem) in      
+  err_result err 
+         (write_lvals (~~direct_call) (p_globs pr)
+                      (with_scs (with_mem st_er m2) scs2) xs vres).
+
+Definition err_reinstate_caller' {E} `{ErrEvent -< E}
+  (fn: funname) (xs: lvals) (vres: values)
+  (st_ee st_er: estate) : itree E ainfo_estate :=
+  f <- err_get_FunDef fn ;;
+  let scs2 := st_ee.(escs) in
+  let m2 := finalize f.(f_extra) st_ee.(emem) in      
+  err_result err 
+       (r_add_info (write_lvals (~~direct_call) (p_globs pr)
+                      (with_scs (with_mem st_er m2) scs2) xs vres)).
+
+
+(** WriteIndex *)
+
+Definition ret_mk_WriteIndex {E} 
+  (x: var_i) (z: Z) (st1: estate) : execT (itree E) estate :=  
+    Ret (r2xs (write_var true x (Vint z) st1)).                             
+
+Definition err_mk_WriteIndex {E} `{ErrEvent -< E}
+  (x: var_i) (z: Z) (st1: estate) : itree E estate :=  
+    err_result err (write_var true x (Vint z) st1).                             
+
+Definition err_mk_WriteIndex0' {E} `{ErrEvent -< E}
+  (x: var_i) (z: Z) (st1: estate) : itree E ainfo_estate :=  
+    err_result err (r_add_info (write_var true x (Vint z) st1)).                             
+Definition err_mk_WriteIndex' {E} `{ErrEvent -< E}
+  (x: var_i) (z: Z) (st: ainfo_estate) : itree E ainfo_estate :=  
+  err_result err
+    (r2air (fst st) (write_var true x (Vint z) (snd st))).                             
+
+(** EvalCond *)
+
+Definition ret_mk_EvalCond {E} 
+  (e: pexpr) (st1: estate) : execT (itree E) bool :=
+   let vv := sem_pexpr true (p_globs pr) st1 e in                               
+   match vv with
+   | Ok (Vbool bb) => ret (ESok bb)
+   | _ => ret (ESerror _ err) end.                       
+
+Definition err_mk_EvalCond {E} `{ErrEvent -< E}
+  (e: pexpr) (st1: estate) : itree E bool :=
+   let vv := sem_pexpr true (p_globs pr) st1 e in                               
+   match vv with
+   | Ok (Vbool bb) => ret bb
+   | _ => throw err end.                       
+
+Definition err_mk_EvalCond' {E} `{ErrEvent -< E}
+  (e: pexpr) (st: ainfo_estate) : itree E ainfo_bool :=
+   let vv := sem_pexpr true (p_globs pr) (snd st) e in                      
+   match vv with
+   | Ok (Vbool bb) => ret (fst st, bb)
+   | _ => throw err end.                       
+
+
+
+(** EvalBound *)
+
+Definition ret_mk_EvalBound {E} 
+  (e: pexpr) (st1: estate) : execT (itree E) Z :=
+   let vv := sem_pexpr true (p_globs pr) st1 e in                               
+   match vv with
+   | Ok (Vint zz) => ret (ESok zz)
+   | _ => ret (ESerror _ err) end.                       
+
+Definition err_mk_EvalBound {E} `{ErrEvent -< E}
+  (e: pexpr) (st1: estate) : itree E Z :=
+   let vv := sem_pexpr true (p_globs pr) st1 e in                               
+   match vv with
+   | Ok (Vint zz) => ret zz
+   | _ => throw err end.                       
+
+Definition err_mk_EvalBound' {E} `{ErrEvent -< E}
+  (e: pexpr) (st: ainfo_estate) : itree E ainfo_Z :=
+   let vv := sem_pexpr true (p_globs pr) (snd st) e in   
+   match vv with
+   | Ok (Vint zz) => ret (fst st, zz)
+   | _ => throw err end.                       
+
+
+(** AssgnE *)
+
+(* terminating *)
+Definition ret_mk_AssgnE {E: Type -> Type} 
+  (x: lval) (tg: assgn_tag) (ty: stype) (e: pexpr) 
+  (st1: estate) : execT (itree E) estate := Ret
+   (r2xs (Let v := sem_pexpr true (p_globs pr) st1 e in 
+    Let v' := truncate_val ty v in
+    write_lval true (p_globs pr) x v' st1)).
+
+Definition err_mk_AssgnE {E: Type -> Type} `{ErrEvent -< E}
+  (x: lval) (tg: assgn_tag) (ty: stype) (e: pexpr) 
+  (st1: estate) : itree E estate :=
+    v <- err_result err (sem_pexpr true (p_globs pr) st1 e) ;;
+    v' <- err_result err (truncate_val ty v) ;;
+    err_result err (write_lval true (p_globs pr) x v' st1).
+
+Definition err_mk_AssgnE' {E: Type -> Type} `{ErrEvent -< E}
+  (x: lval) (tg: assgn_tag) (ty: stype) (e: pexpr) 
+  (st: ainfo_estate) : itree E ainfo_estate :=
+    v <- err_result err (sem_pexpr true (p_globs pr) (snd st) e) ;;
+    v' <- err_result err (truncate_val ty v) ;;
+    err_result err (r2air (fst st)
+                      (write_lval true (p_globs pr) x v' (snd st))).
+
+
+(** OpnE *)
+
+(* terminating *)
+Definition ret_mk_OpnE {E: Type -> Type} 
+  (xs: lvals) (tg: assgn_tag) (o: sopn)
+  (es : pexprs) (st1: estate) : execT (itree E) estate := Ret
+    (r2xs (sem_sopn (p_globs pr) o st1 xs es)).
+
+Definition err_mk_OpnE {E: Type -> Type} `{ErrEvent -< E}
+  (xs: lvals) (tg: assgn_tag) (o: sopn)
+   (es : pexprs) (st1: estate) : itree E estate :=
+    err_result err (sem_sopn (p_globs pr) o st1 xs es).
+
+Definition err_mk_OpnE' {E: Type -> Type} `{ErrEvent -< E}
+  (xs: lvals) (tg: assgn_tag) (o: sopn)
+   (es : pexprs) (st: ainfo_estate) : itree E ainfo_estate :=
+  err_result err (r2air (fst st)
+                    (sem_sopn (p_globs pr) o (snd st) xs es)).
+
+
+(** SyscallE *)
+
+(* terminating *)
+Definition ret_mk_SyscallE {E: Type -> Type}
+  (xs: lvals) (o: syscall_t)
+  (es: pexprs) (st1: estate) : execT (itree E) estate := Ret 
+   (r2xs (Let ves := sem_pexprs true (p_globs pr) st1 es in 
+    Let r3 := exec_syscall st1.(escs) st1.(emem) o ves in 
+    match r3 with
+    | (scs, m, vs) =>
+        write_lvals true (p_globs pr)
+                    (with_scs (with_mem st1 m) scs) xs vs end)).
+
+Definition err_mk_SyscallE {E: Type -> Type} `{ErrEvent -< E}
+  (xs: lvals) (o: syscall_t) (es: pexprs) (st1: estate) :
+  itree E estate :=
+    ves <- err_result err (sem_pexprs true (p_globs pr) st1 es ) ;;
+    r3 <- err_result err (exec_syscall st1.(escs) st1.(emem) o ves) ;;
+    match r3 with
+    | (scs, m, vs) =>
+        err_result err (write_lvals true (p_globs pr)
+                       (with_scs (with_mem st1 m) scs) xs vs) end.
+
+Definition err_mk_SyscallE' {E: Type -> Type} `{ErrEvent -< E}
+  (xs: lvals) (o: syscall_t) (es: pexprs) (st: ainfo_estate) :
+  itree E ainfo_estate :=
+    ves <- err_result err (sem_pexprs true (p_globs pr) (snd st) es ) ;;
+    r3 <- err_result err (exec_syscall (snd st).(escs) (snd st).(emem) o ves) ;;
+    match r3 with
+    | (scs, m, vs) =>
+        err_result err
+          (r2air (fst st) (write_lvals true (p_globs pr)
+                       (with_scs (with_mem (snd st) m) scs) xs vs)) end.
+
+
+(*********************************************************************)
+(*** INTERPRETERS WITH ERROR ******************************)
+
+Definition ainfo_estate_updt (ii: instr_info) (ii_st: ainfo_estate) :
+  ainfo_estate :=
+ let inf' := ainfo_updt ii (fst ii_st) in (inf', snd ii_st). 
+
+(** Auxiliary functions for recursion on list (seq) *)
+Fixpoint st_cmd_map_r {E} (R: instr -> ainfo_estate -> itree E ainfo_estate)
+  (c: cmd) (ii_st: ainfo_estate) : itree E ainfo_estate := 
+  match c with 
+  | nil => Ret ii_st 
+  | i :: c' => ii_st' <- R i ii_st ;; st_cmd_map_r R c' ii_st'
+  end.
+
+Definition isem_foldr_r {E} (R: instr -> ainfo_estate -> itree E ainfo_estate)
+  (c: cmd) : ainfo_estate -> itree E ainfo_estate :=
+  foldr (fun i k s => s' <- R i s ;; k s')
+        (fun s: ainfo_estate => Ret s) c.
+
+(* state events *)
+Variant InstrE : Type -> Type :=
+  | AssgnE : lval -> assgn_tag -> stype -> pexpr -> instr_info ->
+             ainfo_estate -> InstrE ainfo_estate
+  | OpnE : lvals -> assgn_tag -> sopn -> pexprs ->
+           instr_info -> ainfo_estate -> InstrE ainfo_estate
+  | SyscallE : lvals -> syscall_t -> pexprs ->
+               instr_info -> ainfo_estate -> InstrE ainfo_estate
+  | EvalCond (e: pexpr) : instr_info -> ainfo_estate -> InstrE ainfo_bool
+  | EvalBound (e: pexpr) : instr_info -> ainfo_estate -> InstrE ainfo_Z
+  | WriteIndex (x: var_i) (z: Z) :
+    instr_info -> ainfo_estate -> InstrE ainfo_estate
+  | InitState (fn: funname) (vs: values) :
+    instr_info -> ainfo_estate -> InstrE ainfo_estate
+  | RetVal (fn: funname) : instr_info -> ainfo_estate -> InstrE ainfo_values.  
+
+(* mutual recursion events *)
+Variant MREvent : Type -> Type :=
+  | LCode (c: cmd) (st: ainfo_estate) : MREvent ainfo_estate
+  | FCall (xs: lvals) (f: funname) (es: pexprs) (st: ainfo_estate) :
+    MREvent ainfo_estate.
+  
+Local Notation continue_loop st := (ret (inl st)).
+Local Notation exit_loop st := (ret (inr st)).
+Local Notation rec_call := (trigger_inl1). 
+
+Fixpoint eval_for {E} `{ErrEvent -< E} `{InstrE -< E}
+  (R: cmd -> ainfo_estate -> itree E ainfo_estate)                
+  (i: var_i) (c: cmd) (ii: instr_info)
+  (ls: list Z) (ai_st: ainfo_estate) :
+  itree E ainfo_estate :=
+    match ls with
+    | nil => fun ai_st' => ret ai_st'
+    | (w :: ws) => fun ai_st' =>
+                     ai_st1 <- trigger (WriteIndex i w ii ai_st') ;;
+                     ai_st2 <- R c ai_st1 ;;
+                     eval_for R i c ii ws ai_st2
+    end ai_st.
+
+Fixpoint esem_instr {E} `{ErrEvent -< E} `{InstrE -< E}
+  (i : instr) (ai_st: ainfo_estate) :
+  itree (MREvent +' E) ainfo_estate := 
+  let R := st_cmd_map_r esem_instr in
+  let: (MkI ii ir) := i in 
+  match ir with
+  | Cassgn x tg ty e => trigger (AssgnE x tg ty e ii ai_st)
+  | Copn xs tg o es => trigger (OpnE xs tg o es ii ai_st)
+  | Csyscall xs o es => trigger (SyscallE xs o es ii ai_st)
+  | Cif e c1 c2 =>
+      let st := snd ai_st in
+      ib <- trigger (EvalCond e ii ai_st) ;;
+      if snd ib then R c1 (fst ib, st) else R c2 (fst ib, st)                
+  | Cfor i (d, lo, hi) c => 
+      let st := snd ai_st in
+      ai_vlo <- trigger (EvalBound lo ii ai_st) ;;
+      ai_vhi <- trigger (EvalBound hi ii (fst ai_vlo, st)) ;;
+      eval_for R i c ii (wrange d (snd ai_vlo) (snd ai_vhi)) (fst ai_vhi, st)
+  | Cwhile a c1 e inf c2 => 
+      ITree.iter (fun ai_st0 =>
+           ai_st1 <- R c1 ai_st0 ;;          
+           ai_b <- trigger (EvalCond e ii ai_st1) ;;
+           let ai_st1' := (fst ai_b, snd ai_st1) in 
+           if snd ai_b then ai_st2 <- R c2 ai_st1' ;; continue_loop ai_st2
+           else exit_loop ai_st1') ai_st
+  | Ccall xs fn es => rec_call (FCall xs fn es ai_st)      
+  end.
+
+Definition meval_fcall {E} `{ErrEvent -< E} `{InstrE -< E}
+  (xs: lvals) (fn: funname) (es: pexprs) (st0: ainfo_estate) :
+  itree (MREvent +' E) ainfo_estate :=
+  va <- err_eval_Args fn es (snd st0) ;; 
+  st1 <- err_init_state' fn va (snd st0) ;; 
+  c <- err_get_FunCode fn ;; 
+  st2 <- rec_call (LCode c st1) ;; 
+  vs <- err_return_val' fn (snd st2) ;; 
+  err_reinstate_caller' fn xs (snd vs) (snd st2) (snd st0).
+
+Definition meval_cstate {E} `{ErrEvent -< E} `{InstrE -< E} :
+  MREvent ~> itree (MREvent +' E) :=           
+  fun _ fs => match fs with
+              | LCode c st => st_cmd_map_r esem_instr c st
+              | FCall xs fn es st => meval_fcall xs fn es st      
+              end.      
+
+Definition mevalE_cmd {E} `{ErrEvent -< E} `{InstrE -< E}
+  (c: cmd) (st: ainfo_estate) :
+  itree E ainfo_estate :=
+  mrec meval_cstate (LCode c st).
+
+(*
+Definition meval_cmd {E} (c: cmd) (st: estate) : itree E (option estate) := 
+  @interp_Err E estate (mevalE_cmd c st).
+*)
+
+Definition mevalE_fun {E} `{ErrEvent -< E} `{InstrE -< E} :
+  instr_info -> AInfo -> (funname * (values * estate)) -> 
+  itree E (ainfo_values * ainfo_estate) :=
+  fun ii ai fvst =>
+    let '(fn, (va, st)) := fvst in
+    st1 <- trigger (InitState fn va ii (ai, st)) ;;
+    c <- err_get_FunCode fn ;;
+    st2 <- mevalE_cmd c st1 ;;
+    vs <- trigger (RetVal fn ii st2) ;;
+    ret (vs, st2).
+
+Definition meval_fun_ {E} `{ErrEvent -< E} `{InstrE -< E} 
+  (ai: AInfo) (fn: funname) (va: values) (st0: estate) :
+  itree (MREvent +' E) (ainfo_values * ainfo_estate) :=
+  st1 <- err_init_state' fn va st0 ;;
+  c <- err_get_FunCode fn ;;
+  st2 <- rec_call (LCode c st1) ;;
+  vs <- err_return_val' fn (snd st2) ;;
+  ret (vs, st2).
+
+(** InstrE handler *)
+Definition handle_InstrE {E: Type -> Type} 
+  `{ErrEvent -< E} : InstrE ~> itree E :=
+  fun _ e =>
+    match e with
+    | AssgnE xs tg ty es ii st => err_mk_AssgnE' xs tg ty es st
+    | OpnE xs tg o es ii st => err_mk_OpnE' xs tg o es st
+    | SyscallE xs o es ii st => err_mk_SyscallE' xs o es st                              
+    | EvalCond e ii st => err_mk_EvalCond' e st
+    | EvalBound e ii st => err_mk_EvalBound' e st
+    | WriteIndex x z ii st => err_mk_WriteIndex' x z st                              
+    | InitState fn es ii st => err_init_state' fn es (snd st)
+    | RetVal fn ii st => err_return_val' fn (snd st)
+    end.                                            
+        
+Definition ext_handle_InstrE {E: Type -> Type} 
+  `{ErrEvent -< E} : InstrE +' E ~> itree E :=
+  case_ handle_InstrE (id_ E).
+
+(* InstrE interpreter *)
+Definition interp_InstrE {E: Type -> Type} 
+  `{ErrEvent -< E} {A: Type}
+  (t : itree (InstrE +' E) A) : itree E A :=
+  interp ext_handle_InstrE t.
+
+
+End ModularSem.
+
+
+(****************************************************************)
+
+Require Import array_init.
+
+Section ArrayInit.
+
+  (* Analysis info *)
+Local Notation AInfo := Sv.t.  
+Context (empty_ainfo : AInfo).
+Context (ainfo_updt : instr_info -> AInfo -> AInfo).
+
+Notation ainfo_estate := (AInfo * estate)%type.
+Notation ainfo_bool := (AInfo * bool)%type.
+Notation ainfo_Z := (AInfo * Z)%type.
+Notation ainfo_values := (AInfo * values)%type.
+
+
+(*
+Check @add_init_i.
+@add_init_i : forall (asm_op : Type) (asmop : asmOp asm_op),
+       Sv.t -> instr -> cmd * Sv.t
+*)
+
+Definition add_init_Aux_g (ai: AInfo) (ii: instr_info) (ir: instr_r) :
+  (cmd * Sv.t) := 
+    let Wi := write_i ir in
+    let Ri := read_i ir in
+    let extra := Sv.union Wi Ri in
+    (add_init (ii_with_location ii) ai extra (MkI ii ir), Sv.union ai Wi).
+
+
+(** InstrE handler for Array Init *)
+Definition handle_InstrE_init {E: Type -> Type} 
+  `{ErrEvent -< E} `{InstrE AInfo -< E} : InstrE AInfo ~> itree E :=
+  fun _ e =>
+    match e with
+    | AssgnE xs tg ty es ii ai_st =>
+        let ir := Cassgn xs tg ty es in
+        let '(cmd1, ai1) := add_init_Aux_g (fst ai_st) ii ir in
+        @mevalE_cmd AInfo empty_ainfo _ _ _ cmd1 (ai1, snd ai_st)
+    | OpnE xs tg o es ii ai_st =>
+        let ir := Copn xs tg o es in
+        let '(cmd1, ai1) := add_init_Aux_g (fst ai_st) ii ir in
+        @mevalE_cmd AInfo empty_ainfo _ _ _ cmd1 (ai1, snd ai_st)
+    | SyscallE xs o es ii ai_st => 
+        let ir := Csyscall xs o es in
+        let '(cmd1, ai1) := add_init_Aux_g (fst ai_st) ii ir in
+        @mevalE_cmd AInfo empty_ainfo _ _ _ cmd1 (ai1, snd ai_st)
+   | _ => throw err
+    end.             
+
+(* Remark: R does not use ainfo, which comes from aic. the monad
+   shoudl be fixed. *)
+Definition isem_foldr2 {E} 
+  (R: instr -> ainfo_estate -> itree E ainfo_estate)
+  (aic: (cmd * AInfo)) : ainfo_estate -> itree E ainfo_estate :=
+  foldr (fun i k (s: ainfo_estate) => s' <- R i (snd aic, snd s) ;; k s')
+        (fun s: ainfo_estate => Ret s) (fst aic).
+
+(* *)
+Definition isem_foldr1 {E} 
+  (R: instr -> estate -> itree E estate)
+  (aic: (cmd * AInfo)) : estate -> itree E ainfo_estate :=
+  foldr (fun i k (s: estate) => s' <- R i s ;; k s')
+        (fun s: estate => Ret (snd aic, s)) (fst aic).
+
+Fixpoint st_cmd_map_r_AI2 {E}
+  (R: instr -> ainfo_estate -> itree E ainfo_estate)
+  (c: cmd) (ii_st: ainfo_estate) : itree E ainfo_estate := 
+  match c with 
+  | nil => Ret ii_st 
+  | i :: c' =>
+      ii_st' <- isem_foldr2 R (add_init_i (fst ii_st) i) ii_st ;;
+      st_cmd_map_r_AI2 R c' ii_st'
+  end.
+
+Fixpoint st_cmd_map_r_AI1 {E} (R: instr -> estate -> itree E estate)
+  (c: cmd) (ii_st: ainfo_estate) : itree E ainfo_estate := 
+  match c with 
+  | nil => Ret ii_st 
+  | i :: c' => ii_st' <- isem_foldr1 R (add_init_i (fst ii_st) i) (snd ii_st) ;;
+               st_cmd_map_r_AI1 R c' ii_st'
+  end.
+
+(*   
+initialization of I in a function call: 
+let I := vrvs [seq (Lvar i) | i <- f_params fd] in
+*)
+Definition meval_cstate_AI2 {E} {X1: ErrEvent -< E} {X2: InstrE AInfo -< E} :
+  MREvent AInfo ~> itree (MREvent AInfo +' E) :=           
+  fun _ fs => match fs with
+              | LCode c ai_st => st_cmd_map_r_AI2
+                                   (@esem_instr AInfo E X1 X2) c ai_st
+              | FCall xs fn es ai_st =>
+                  @meval_fcall AInfo empty_ainfo E X1 X2 xs fn es ai_st      
+              end.      
+
+
+End ArrayInit.
+
+End WSW.
+
